reducible is for valid_exec now (not frag) + progress in reduction proof

txn-data-consistency/Reductions.thy
@@ -84,21 +84,26 @@ lemma reduce_frag_plus_last_state_equiv: \<open>E: ef1 \<rhd>\<^sup>+ ef2 \<Long
 
 inductive reducible :: "('e, 's) ES \<Rightarrow> ('e, 's) exec_frag set \<Rightarrow> bool" for E Good where
   reducibleI: 
-    "\<lbrakk> \<And>ef. \<lbrakk> valid_exec_frag E ef; ef \<notin> Good \<rbrakk> \<Longrightarrow> \<exists>ef' \<in> Good. E: ef \<rhd>\<^sup>+ ef' \<rbrakk> 
+    "\<lbrakk> \<And>ef. \<lbrakk> valid_exec E ef; ef \<notin> Good \<rbrakk> \<Longrightarrow> \<exists>ef' \<in> Good. E: ef \<rhd>\<^sup>+ ef' \<rbrakk> 
      \<Longrightarrow> reducible E Good"
+
+inductive reducible_frag :: "('e, 's) ES \<Rightarrow> ('e, 's) exec_frag set \<Rightarrow> bool" for E Good where
+  reducible_fragI: 
+    "\<lbrakk> \<And>ef. \<lbrakk> valid_exec_frag E ef; ef \<notin> Good \<rbrakk> \<Longrightarrow> \<exists>ef' \<in> Good. E: ef \<rhd>\<^sup>+ ef' \<rbrakk> 
+     \<Longrightarrow> reducible_frag E Good"
 
 
 subsection \<open>Reduction proof rules\<close>
 
-lemma reducible_to_Good_exec_frag:
+lemma reducible_to_Good_exec:
   assumes
     \<open>wf R\<close>
-    \<open>\<And>ef. \<lbrakk> valid_exec_frag E ef; ef \<notin> Good \<rbrakk> \<Longrightarrow> (\<exists>ef'. E: ef \<rhd> ef' \<and> (ef' \<in> Good \<or> (ef', ef) \<in> R))\<close>
+    \<open>\<And>ef. \<lbrakk> valid_exec E ef; ef \<notin> Good \<rbrakk> \<Longrightarrow> (\<exists>ef'. E: ef \<rhd> ef' \<and> (ef' \<in> Good \<or> (ef', ef) \<in> R))\<close>
   shows
     \<open>reducible E Good\<close>
 proof 
   fix ef
-  assume \<open>valid_exec_frag E ef\<close> \<open>ef \<notin> Good\<close>
+  assume \<open>valid_exec E ef\<close> \<open>ef \<notin> Good\<close>
   with \<open>wf R\<close> show \<open>\<exists>ef' \<in> Good. E: ef \<rhd>\<^sup>+ ef'\<close> 
   proof (induction ef rule: wf_induct_rule)
     case (less x)
@@ -110,7 +115,7 @@ proof
     next
       case False
       then obtain a where "a \<in> Good" and "E: ef' \<rhd>\<^sup>+ a"
-        using less ef' by (blast dest: reduce_frag_valid)
+        using less ef' by (blast dest: reduce_exec_reduced_valid)
       then show ?thesis using \<open>E: x \<rhd> ef'\<close> by (blast intro: tranclp_into_tranclp2)
     qed
   qed
@@ -128,7 +133,7 @@ lemma reach_reduced:
     \<open>s \<in> ef_last`Good\<close>
   using assms
 proof -
-  from \<open>reach E s\<close> obtain s0 efl where *: \<open>valid_exec_frag E (Exec_frag s0 efl s)\<close> 
+  from \<open>reach E s\<close> obtain s0 efl where *: \<open>valid_exec E (Exec_frag s0 efl s)\<close> 
     by (auto simp add: reach_last_exec)
   then show ?thesis
   proof (cases "Exec_frag s0 efl s \<in> Good")
@@ -203,7 +208,7 @@ lemma left_commute_diamond:
   by (auto simp add: left_commute_def)
 
 text \<open>Commute transitions in execution fragments. This lemma might be useful for establishing
-the main premise of the rule @{thm reducible_to_Good_exec_frag} given that we know that
+the main premise of the rule @{thm reducible_to_Good_exec} given that we know that
 two events left-commute.\<close>
 
 lemma reduce_frag_left_commute:
@@ -314,7 +319,7 @@ lemma exec_frag_good_ects:
 
 lemma reducible_exec_frag:
   assumes
-    \<open>valid_exec_frag E ef\<close>
+    \<open>valid_exec E ef\<close>
     \<open>ef \<notin> Good_wrt f\<close>
     \<open>wf (measure_rel f)\<close>
   shows
@@ -326,7 +331,7 @@ lemma reducible_exec_frag:
 lemma reducible_to_Good_wrt_f_exec_frag: 
   fixes f :: \<open>'e \<Rightarrow> 'a :: linorder option\<close>
   shows \<open>reducible E (Good_wrt f)\<close>
-  by (auto intro: reducible_to_Good_exec_frag [OF _ reducible_exec_frag])
+  by (auto intro: reducible_to_Good_exec [OF _ reducible_exec_frag])
 
 
 end
